Chapter 10.2 - The Hot Water Heater Problem Revisited
========================================================
author: Clayton Johnson
date: 
autosize: true

Example 10.3: Solving Diff. Eqs with Integrating Factors
========================================================
We need to solve equation 10.7 (below):

$$
\frac{dU}{dt} = \beta - \alpha U,
$$

where 

$$
\alpha = \frac{hS}{cm}, \\
\beta = \frac{q+hSu_s}{cm}, \\
U(0) = u_0.
$$

Example 10.3: Solving Diff. Eqs with I.F. 
========================================================
$$
\frac{dU}{dt} + \alpha U = \beta,
$$

First-order linear differential equation. We can solve using integrating factor technique, producing the integrating factor,

$$
R(t) = e^{\int_{0}^{t} \alpha dt} = e^{\alpha t}.
$$

Example 10.3: Solving Diff. Eqs with I.F. 
========================================================
Rewriting the differential equation, we have that

$$
\begin{align*}
\frac{dU}{dt} + \alpha U &= \beta, \\
\frac{dU}{dt}\times e^{\alpha t} + \alpha U \times e^{\alpha t} &= \beta \times e^{\alpha t}, \\
e^{\alpha t} \frac{dU}{dt} + \frac{d}{dt}\left( e^{\alpha t} \right) U &= \beta e^{\alpha t}, \\
\frac{d}{dt} \left( U e^{\alpha t} \right) &= \beta e^{\alpha t}, \text{ using the chain rule.}
\end{align*}
$$

Example 10.3: Solving Diff. Eqs with I.F. 
========================================================
Integrating both sides with respect to $t$,

$$
e^{\alpha t}U = \frac{\beta}{\alpha}e^{\alpha t} + K, \\
\text{and } U = \frac{\beta}{\alpha} + Ke^{-\alpha t},
$$

where $K$ is the constant of integration.

Example 10.3: Solving Diff. Eqs with I.F. 
========================================================

Applying the initial condition $U(0)=u_0$, we find that $K = u_0 - \frac{\beta}{\alpha}$. Hence, the solution is,

$$
U = u_0e^{-\alpha t} + \frac{\beta}{\alpha}(1-e^{-\alpha t}).
$$

Substituting $\alpha$ and $\beta$ gives equation 10.8 (below),

$$
U(t) = \left( u_0 - u_s - \frac{q}{hS} \right) e^{- \frac{hS}{cm} t } + u_s + \frac{q}{hS}.
$$
